### 4.4.1
***
For each of the following grammars, devise predictive parsers and show the parsing tables. You may left-factor and/or eliminate left-recursion from your grammars first.

a) The grammar of Exercise 4.2.2(a).

b) The grammar of Exercise 4.2.2(b).

c) The grammar of Exercise 4.2.2(c).

d) The grammar of Exercise 4.2.2(d).

e) The grammar of Exercise 4.2.2(e).

f) The grammar of Exercise 4.2.2(g).

### `Answer`
a) ```S -> 0 S 1 | 0 1```

Left Factoring,
```
S  -> 0 S'
S' -> S 1 | 1
```

Eliminating Left Recursion,
```
S  -> 0 S'
S' -> 0 S' 1 | 1
```

```
FIRST(S) = {0}
FIRST(S') = {0, 1}

FOLLOW(S) = {$}
FOLLOW(S') = {$, 1}
```

| NON TERMINAL |                      |  INPUT SYMBOL |         |
|--------------|----------------------|---------------|---------|
|              |        ```0```       |    ```1```    | ```$``` |
|    ```S```   |    ```S -> 0 S'```   |               |         |
|   ```S'```   |  ```S' -> 0 S' 1 ``` | ```S' -> 1``` |         |


b) ```S -> + S S | * S S | a```

```
FIRST(S) = {+, *, a}

FOLLOW(S) = {$, +, *, a}
```

| NON TERMINAL |                  |   INPUT SYMBOL   |               |         |
|--------------|------------------|------------------|---------------|---------|
|              |      ```+```     |      ```*```     |    ```a```    | ```$``` |
|    ```S```   | ```S -> + S S``` | ```S -> * S S``` |  ```S -> a``` |         |

c) ```S -> S ( S ) S | ε```

Eliminating Left Recursion,
```
S  -> S'
S' -> ( S ) S S' | ε
```

```
FIRST(S) = {(, ε}
FIRST(S') = {(, ε}

FOLLOW(S) = {$, ), (}
FOLLOW(S') = {$, ), (}
```

| NON TERMINAL |                        |  INPUT SYMBOL |               |
|--------------|------------------------|---------------|---------------|
|              |         ```(```        |    ```)```    |    ```$```    |
|    ```S```   |      ```S -> S'```     |  ```S -> ε``` |  ```S -> ε``` |
|              |      ```S -> ε```      |               |               |
|   ```S'```   | ```S' -> ( S ) S S'``` | ```S' -> ε``` | ```S' -> ε``` |
|              |      ```S' -> ε```     |               |               |


d) ```S -> S + S | S S | ( S ) | S * | a```

Left Factoring,
```
S  -> S S' | ( S ) | a
S' -> + S | S | *
```

Eliminating Left Recursion,
```
S   -> ( S ) S'' | a S''
S'' -> S' S'' | ε
S'  -> + S | ( S ) S'' | a S'' | ε
```

```
FIRST(S) = {(, a}
FIRST(S'') = {+, (, a, ε}
FIRST(S') = {+, (, a, ε}

FOLLOW(S) = {$, ), +, (, a}
FOLLOW(S'') = {$, ), +, (, a}
FOLLOW(S') = {+, (, a, $, )}
```

| NON TERMINAL |                       |                |     INPUT SYMBOL    |                     |                |
|--------------|-----------------------|----------------|---------------------|---------------------|----------------|
|              |         ```(```       |     ```)```    |       ```a```       |       ```+```       |     ```$```    |
|    ```S```   |  ```S -> ( S ) S''``` |                |   ```S -> a S''```  |                     |                |
|   ```S''```  |  ```S'' -> S' S''```  | ```S'' -> ε``` | ```S'' -> S' S''``` | ```S'' -> S' S''``` | ```S'' -> ε``` |
|              |     ```S'' -> ε```    |                |    ```S'' -> ε```   |    ```S'' -> ε```   |                |
|   ```S'```   | ```S' -> ( S ) S''``` |  ```S' -> ε``` |  ```S' -> a S''```  |   ```S' -> + S```   |  ```S' -> ε``` |
|              |     ```S' -> ε```     |                |    ```S' -> ε```    |    ```S' -> ε```    |                |

e) ```S -> ( L ) | a``` and ```L -> L , S | S```

Eliminating Left Recursion,
```
S  -> ( L ) | a
L  -> ( L ) L' | a L'
L' -> , ( L ) L' | , a L' | ε
```

```
FIRST(S) = {(, a}
FIRST(L) = {(, a}
FIRST(L') = {,, ε}

FOLLOW(S) = {$}
FOLLOW(L) = {)}
FOLLOW(L') = {)}
```

| NON TERMINAL |                       |                |     INPUT SYMBOL    |                        |                |
|--------------|-----------------------|----------------|---------------------|------------------------|----------------|
|              |         ```(```       |     ```)```    |       ```a```       |         ```,```        |     ```$```    |
|    ```S```   |    ```S -> ( L ) ```  |                |     ```S -> a ```   |                        |                |
|    ```L```   |  ```L -> ( L ) L'```  |                |   ```L -> a L'```   |                        |                |
|   ```L'```   |                       |  ```L' -> ε``` |                     | ```L' -> , ( L ) L'``` |                |
|              |                       |                |                     |   ```L' -> , a L'```   |                |

f)
```
  bexpr -> bexpr or bterm | bterm
  bterm -> bterm and bfactor | bfactor
bfactor -> not bfactor | ( bexpr ) | true | false
```

Eliminating Left Recursion,
```
  bexpr -> bterm bexpr'
 bexpr' -> or bterm bexpr' | ε
  bterm -> bfactor bterm'
 bterm' -> and bfactor bterm' | ε
bfactor -> not bfactor | ( bexpr ) | true | false
```

```
FIRST(bexpr) = {not, (, true, false}
FIRST(bexpr') = {or, ε}
FIRST(bterm) = {not, (, true, false}
FIRST(bterm') = {and, ε}
FIRST(bfactor) = {not, (, true, false}

FOLLOW(bexpr) = {$, )}
FOLLOW(bexpr') = {$, )}
FOLLOW(bterm) = {or, $, )}
FOLLOW(bterm') = {or, $, )]
FOLLOW(bfactor) = {and, or, $, )}
```

|  NON TERMINAL |                                 |                                    |                               |          INPUT SYMBOL         |                         |                               |                               |                         |
|---------------|---------------------------------|------------------------------------|-------------------------------|-------------------------------|-------------------------|-------------------------------|-------------------------------|-------------------------|
|               |             ```or```            |              ```and```             |           ```not```           |            ```(```            |         ```)```         |           ```true```          |          ```false```          |         ```$```         |
|  ```bexpr```  |                                 |                                    |  ```bexpr -> bterm bexpr'```  |  ```bexpr -> bterm bexpr'```  |                         |  ```bexpr -> bterm bexpr'```  |  ```bexpr -> bterm bexpr'```  |                         |
|  ```bexpr'``` | ```bexpr' -> or bterm bexpr'``` |                                    |                               |                               |    ```bexpr' -> ε```    |                               |                               |    ```bexpr' -> ε```    |
|  ```bterm```  |                                 |                                    | ```bterm -> bfactor bterm'``` | ```bterm -> bfactor bterm'``` |                         | ```bterm -> bfactor bterm'``` | ```bterm -> bfactor bterm'``` |                         |
|  ```bterm'``` |         ```bterm' -> ε```       | ```bterm' -> and bfactor bterm'``` |                               |                               |    ```bterm' -> ε```    |                               |                               |    ```bterm' -> ε```    |
| ```bfactor``` |                                 |                                    |  ```bfactor -> not bfactor``` |   ```bfactor -> ( bexpr )```  |                         |     ```bfactor -> true```     |     ```bfactor -> false```    |                         |

### 4.4.3
***
Compute FIRST and FOLLOW for the grammar of Exercise 4.2.1.

### `Answer`
```S -> S S + | S S * | a```

```
FIRST(S) = {a}

FOLLOW(S) = {$, a, +, *}
```

### 4.4.4
***
Compute FIRST and FOLLOW for each of the grammars of Exercise 4.2.2.

### `Answer`
a) ```S -> 0 S 1 | 0 1```

```
FIRST(S) = {0}

FOLLOW(S) = {$, 1}
```

b) ```S -> + S S | * S S | a```

```
FIRST(S) = {+, *, a}

FOLLOW(S) = {$, +, *, a}
```

c) ```S -> S ( S ) S | ε```

```
FIRST(S) = {ε}

FOLLOW(S) = {$, (, )}
```

d) ```S -> S + S | S S | ( S ) | S * | a```

```
FIRST(S) = {(, a}

FOLLOW(S) = {$, +, (, a, ), *}
```

e) ```S -> ( L ) | a``` and ```L -> L , S | S```

```
FIRST(S) = {(, a}
FIRST(L) = {(, a}

FOLLOW(S) = {$, ), ,}
FOLLOW(L) = {), ,)
```

f) ```S -> a S b S | b S a S | ε```

```
FIRST(S) = {a, b, ε}

FOLLOW(S) = {$, b, a}
```

g)
```
  bexpr -> bexpr or bterm | bterm
  bterm -> bterm and bfactor | bfactor
bfactor -> not bfactor | ( bexpr ) | true | false
```

```
FIRST(bexpr) = {not, (, true, false}
FIRST(bterm) = {not, (, true, false}
FIRST(bfactor) = {not, (, true, false}

FOLLOW(bexpr) = {$, or, )}
FOLLOW(bterm) = {$, or, ), and}
FOLLOW(bfactor) = {$, or, ), and}
```
