### 2.3.1
***
Construct recursive-descent parsers, starting with the following grammars:
```
a) S -> + S S | - S S | a

b) S -> S ( S ) S | Îµ

c) S -> 0 S 1 | 0 1
```

### `Answer`
a)
```
void S() {
      switch ( lookahead ) {
      case '+':
            match('+'); S(); S(); break;
      case '-':
            match('-'); S(); S(); break;
      case 'a':
            match('a'); break;
      default:
            report("syntax error");
      }
}

void match(terminal t) {
      if (lookahead == t) lookahead = nextTerminal;
      else report("syntax error");
}
```

b)
```
void S() {
      if (lookahead == '(')
            match('('); S(); match(')'); S(); break;
}

void match(terminal t) {
      if (lookahead == t) lookahead = nextTerminal;
      else report("syntax error");
}
```

c)
```
void S() {
      if (lookahead == '0') {
            match('0');
            if (lookahead == '1')
                  match('1'); 
            else
                  S(); match('1'); break;
      } else report("syntax error");
}

void match(terminal t) {
      if (lookahead == t) lookahead = nextTerminal;
      else report("syntax error");
}
```
